src/zfc.lean
@@ -63,114 +63,12 @@ def functional {n} (c : bounded_formula L_ZFC (n+2)) : bounded_formula L_ZFC n :
 def subset : bounded_formula L_ZFC 2 := ∀' (&0 ∈' &1 ⟹ &0 ∈' &2)
 def is_emptyset : bounded_formula L_ZFC 1 := ∼ ∃' (&0 ∈' &1)
 
-def pair : bounded_formula L_ZFC 3 := (&0 ≃ &1 : bounded_formula L_ZFC 3) ⊔ (&0 ≃ &2 : bounded_formula L_ZFC 3)
+def pair : bounded_formula L_ZFC 3 :=
+(&0 ≃ &1 : bounded_formula L_ZFC 3) ⊔ (&0 ≃ &2 : bounded_formula L_ZFC 3)
 def singl : bounded_formula L_ZFC 2 := &0 ≃ &1
 def binary_union : bounded_formula L_ZFC 3 := &0 ∈' &1 ⊔ &0 ∈' &2
 def succ : bounded_formula L_ZFC 2 := (&0 ≃ &1 : bounded_formula L_ZFC 2) ⊔ &0 ∈' &1
 
-def ordered_pair : bounded_formula L_ZFC 3 := ∀'(&0 ∈' &1 ⇔ (&0 ≃ &3 : bounded_formula L_ZFC 4) ⊔ ∀'(&0 ∈' &1 ⇔ pair ↑' 1 # 1 ↑' 1 # 1))
-
--- &0 is an ordered pair of &2 and &1 (z = ⟨x, y⟩)
-
-def ordered_pair' : bounded_formula L_ZFC 3 := ∀'(&0 ∈' &3 ⇔ (&0 ≃ &2 : bounded_formula L_ZFC 4) ⊔ ∀'(&0 ∈' &1 ⇔ (pair ↑' 1 # 1).cast(lift_cast)))
--- &2 is an ordered pair of &1 and &0 (x = ⟨y,z⟩)
--- TODO: Make defns like this unnecessary (current effort is subst_var_* in fol.lean)
-
-def is_ordered_pair : bounded_formula L_ZFC 1 := ∃' ∃' ordered_pair
---&0 is an ordered pair of some two elements--
-
-local notation h :: t  := dvector.cons h t
-local notation `[` l:(foldr `, ` (h t, dvector.cons h t) dvector.nil `]`) := l
-
-def relation : bounded_formula L_ZFC 1 := ∀' ((&0 ∈' &1) ⟹ is_ordered_pair ↑' 1 # 1)
---&0 is a relation (is a set of ordered pairs)
-
-def relation' : bounded_formula L_ZFC 1 := ∀' (((&0 ∈' &1) : bounded_formula L_ZFC 2) ⟹ (is_ordered_pair ⊚ [0]))
-
-lemma chk: relation = relation' := sorry
---ideally this should be by refl. Comment out the set_option above the defn of subst_var_bounded_formula to see the snag
-
-
-def function : bounded_formula L_ZFC 1 := relation ⊓ ∀'∀'∀'∀'∀'(&1 ∈' &5 ⊓ ordered_pair ↑' 1 # 3 ↑' 1 # 1 ↑' 1 # 0 ⊓ ((&0 ∈' &5 : bounded_formula L_ZFC 6) ⊓ (ordered_pair ↑' 1 # 2 ↑' 1 # 1).cast(lift_cast)) ⟹ (&3 ≃ &2 : bounded_formula L_ZFC 6))
--- X is a function iff X is a relation and the following holds:
--- ∀x ∀y ∀z ∀w ∀t, ((w ∈ X) ∧ (w = ⟨x, y⟩) ∧ (z ∈ X) ∧ (z = ⟨x, z⟩ ))) →  y = z
-
-def function' : bounded_formula L_ZFC 1 := relation ⊓ ∀'∀'∀'∀'∀'(((&1 ∈' &5 : bounded_formula L_ZFC 6) ⊓ (ordered_pair ⊚ [1,3,4]) ⊓ ((&0 ∈' &5 : bounded_formula L_ZFC 6) ⊓ (ordered_pair ⊚ [0,2,4]))) ⟹ (&3 ≃ &2 : bounded_formula L_ZFC 6))
-
-
-def fn_app : bounded_formula L_ZFC 3 := ∃'(&0 ∈' &3 ⊓ ∀'(&0 ∈' &1 ⇔ ((&0 ≃ &3): bounded_formula L_ZFC 5) ⊔ (pair ↑' 1 # 1).cast(lift_cast)))
--- ⟨&1, &0⟩ ∈ &2
--- &0 = &2(&1)
-
-def fn_domain : bounded_formula L_ZFC 2 := ∀'(&0 ∈' &2 ⇔ ∃'∃'(ordered_pair ↑' 1 # 1 ↑' 1 # 1 ⊓ &0 ∈' &3))
--- &1 is the domain of &0
-
-def fn_range : bounded_formula L_ZFC 2 := ∀'(&0 ∈' &2 ⇔ ∃'∃'(∀'(&0 ∈' &1 ⇔ (&0 ≃ &2 : bounded_formula L_ZFC 6) ⊔ (pair ↑' 1 # 1).cast(lift_cast)) ⊓ &0 ∈' &3))
---&1 is the range of &0
-
-def inverse_relation : bounded_formula L_ZFC 2 := ∀'(&0 ∈' &1 ⇔ ∃'∃'(∃'(∀'(&0 ∈' &1 ⇔ (&0 ≃ &2 : bounded_formula L_ZFC 7) ⊔ (pair ↑' 1 # 1).cast(lift_cast)) ⊓ &0 ∈' &5 : bounded_formula L_ZFC 6)) ⊓ (ordered_pair'.cast(lift_cast)))
--- &0 is the inverse relation of &1
-
-def function_one_one : bounded_formula L_ZFC 1 := function ⊓ ∀' (inverse_relation ⟹ function.cast(lift_cast))
-
-def irreflexive_relation : bounded_formula L_ZFC 2 :=  (∀'(&0 ∈' &2 ⟹ (∀'(∀'(&0 ∈' &1) ⇔ ((&0 ≃ &2 : bounded_formula L_ZFC 4) ⊔ ∀'(&0 ∈' &1 ⇔ (&0 ≃ &3 : bounded_formula L_ZFC 5))) ⟹ ∼(&0 ∈' &3))))) ⊓ relation.cast(lift_cast)
--- &0 is an irreflexive relation on &1
-
-def transitive_relation : bounded_formula L_ZFC 2 := ((∀'∀'∀'((((&2 ∈' &4 : bounded_formula L_ZFC 5) ⊓ (&1 ∈' &4)) ⊓ (&0 ∈' &4)) ⊓ ∃'((ordered_pair ↑' 1 # 1).cast(lift_cast) ⊓ (&0 ∈' &4 : bounded_formula L_ZFC 6)) ⊓ ∃'(ordered_pair.cast(lift_cast) ⊓ &0 ∈' &4 : bounded_formula L_ZFC 6) ⟹ ∃'((ordered_pair ↑' 1 # 2).cast(lift_cast) ⊓ &0 ∈' &4 : bounded_formula L_ZFC 6)))) ⊓ relation.cast(lift_cast)
---&0 is a transitive relation on &1
--- X Tr Y iff X is a relation and the following holds:
--- ∀u ∀v ∀w, (u ∈ Y ∧ v ∈ Y ∧ w ∈ Y ∧ ⟨u, v⟩ ∈ X ∧ ⟨v,w⟩ ∈ X) → ⟨u,w⟩ ∈ X
-
-def partial_order_zfc : bounded_formula L_ZFC 2 := irreflexive_relation ⊓ transitive_relation
-
-def connected_relation : bounded_formula L_ZFC 2 := relation ↑' 1 # 1 ⊓ ∀'∀'((bd_and (bd_and (&0 ∈' &3) (&1 ∈' &3)) ∼(bd_equal &0 &1)) ⟹ ∃'((&0 ∈' &3 : bounded_formula L_ZFC 5) ⊓ ((ordered_pair ↑' 1 # 3 ↑' 1 # 3) ⊔ ∀'(&0 ∈' &1 ⇔ (&0 ≃ &2 : bounded_formula L_ZFC 6) ⊔ (pair ↑' 1 # 1).cast(lift_cast)))))
---&0 is a connected relation on &1
--- X Con Y iff Rel(X) and ∀u ∀v (u ∈ Y ∧ v ∈ Y ∧ u ≠ v) → ⟨u,v⟩ ∈ X ∨ ⟨v, u⟩ ∈ X
-
-def total_order : bounded_formula L_ZFC 2 := irreflexive_relation ⊓ transitive_relation ⊓ connected_relation
-
-def well_order : bounded_formula L_ZFC 2 := irreflexive_relation ⊓ ∀'(subset ↑' 1 # 1 ⊓ ∃'(&0 ∈' &1) ⟹ ∃'(&0 ∈' &1 ⊓ ∀'(((&0 ∈' &2) ⊓  ∼(&0 ≃ &1 : bounded_formula L_ZFC 5)) ⟹ ∃'(ordered_pair.cast(lift_cast) ⊓ (&0 ∈' &4 : bounded_formula L_ZFC 6)) ⊓ ∼∃'(∀'(&0 ∈' &1 ⇔ (( &0 ≃ &2 : bounded_formula L_ZFC 7) ⊔ (pair ↑' 1 # 1).cast(lift_cast) )) ⊓ &0 ∈' &4))))
--- &0 well-orders &1
-
-def membership_relation : bounded_formula L_ZFC 1 := relation ⊓ ∀'(&0 ∈' &1 ⇔ ∃'∃'∀'(&0 ∈' &3 ⇔ ((bd_equal &0  &2) ⊔ pair ↑' 1 # 3 ↑' 1 # 3) ⊓ &2 ∈' &1))
--- &0 is E, the membership relation {⟨x,y⟩ | x ∈ y}
-
-def transitive_zfc : bounded_formula L_ZFC 1 := ∀' ((&0 ∈' &1) ⟹ subset)
---&0 is transitive
-
-def fn_zfc_equiv : bounded_formula L_ZFC 3 := ((function_one_one.cast(lift_cast)) ⊓ (fn_domain ↑' 1 # 1)) ⊓ (fn_range ↑' 1 # 2)
-
-def zfc_equiv : bounded_formula L_ZFC 2 := ∃' fn_zfc_equiv
---&0 ≃ &1, i.e. they are equinumerous
-
-def is_powerset : bounded_formula L_ZFC 2 := ∀' ((&0 ∈' &2) ⇔ subset ↑' 1 # 2)
---&1 is P(&0)
-
-def is_suc_of : bounded_formula L_ZFC 2 := ∀' ((&0 ∈' &2) ⇔ ((&0 ∈' &1) ⊔ ( &0 ≃ &1 : bounded_formula L_ZFC 3)))
--- &1 = succ(&0)
-
-def is_ordinal : bounded_formula L_ZFC 1 := (∀' ((membership_relation.cast(lift_cast)) ⟹ well_order)) ⊓ transitive_zfc
-
-def is_suc_ordinal : bounded_formula L_ZFC 1 := is_ordinal ⊓ ∃' is_suc_of
---&0 is a successor ordinal
-
-def ordinal_lt : bounded_formula L_ZFC 2 := (is_ordinal.cast(lift_cast)) ⊓ (is_ordinal ↑' 1 # 0) ⊓ (&0 ∈' &1)
--- &0 < &1
-
-def ordinal_le : bounded_formula L_ZFC 2 := ordinal_lt ⊔ (bd_equal &0 &1)
--- &0 ≤ &1
-
-def is_first_infinite_ordinal : bounded_formula L_ZFC 1 := ∀' ((&0 ∈' &1) ⇔ (((is_emptyset ⊔ is_suc_ordinal)↑' 1 # 1) ⊓ ∀'((&0 ∈' &1) ⟹ ((is_emptyset ⊔ is_suc_ordinal).cast(lift_cast)))))
---&0 = ω
-
-def is_uncountable_ordinal : bounded_formula L_ZFC 1 := ∀' ((is_first_infinite_ordinal.cast(lift_cast)) ⟹ ∀' (subset.cast(lift_cast) ⟹(∼(zfc_equiv ↑' 1 # 1))))
---&0 ≥ ω₁
-
-def is_first_uncountable_ordinal : bounded_formula L_ZFC 1 := is_uncountable_ordinal ⊓ (∀' ((is_uncountable_ordinal ↑' 1 # 1) ⟹ ordinal_le))
---&0 = ω₁
-
-/- Statement of CH -/
-def continuum_hypothesis : sentence L_ZFC := ∀' ∀'  ((∃'((is_first_infinite_ordinal ↑' 1 # 1 ↑' 1 # 1) ⊓ (is_powerset ↑' 1 # 2)) ⊓ (is_first_uncountable_ordinal ↑' 1 #0)) ⟹ zfc_equiv)
 
 def axiom_of_extensionality : sentence L_ZFC := ∀' ∀' (∀' (&0 ∈' &1 ⇔ &0 ∈' &2) ⟹ &0 ≃ &1)
 def axiom_of_union : sentence L_ZFC := ∀' (small ∃' (&1 ∈' &0 ⊓ &0 ∈' &2))
@@ -183,25 +81,178 @@ def axiom_of_powerset : sentence L_ZFC :=
 ∀' small subset
 def axiom_of_infinity : sentence L_ZFC :=
 --∃ y ((∃ y', y = ∅ ∧ y' ∈ y) ∧ ∀ z (z ∈ y → ∃w(z ∈ w ∧ w ∈ y)))
-∃' ((∃' (bd_and (is_emptyset ↑' 1 # 1) (&0 ∈' &1) : bounded_formula L_ZFC 2)) ⊓ ∀'(&0 ∈' &1 ⟹ ∃' (bd_and (&1 ∈' &0) (&0 ∈' &2))))
+∃' ((∃' (bd_and (is_emptyset ↑' 1 # 1) (&0 ∈' &1) : bounded_formula L_ZFC 2)) ⊓
+  ∀'(&0 ∈' &1 ⟹ ∃' (bd_and (&1 ∈' &0) (&0 ∈' &2))))
 
 def axiom_of_infinity' : sentence L_ZFC :=
-∃' ∀' ((is_emptyset.cast (lift_cast)  ⟹ (&0 ∈' &1) : bounded_formula L_ZFC 2) ⊓ (∀' (&0 ∈' &2 ⟹ (∃' ((&1 ∈' &0).cast (lift_cast) ⊓ (&0 ∈' &3) : bounded_formula L_ZFC 4)))))
-
-def axiom_of_choice : sentence L_ZFC := ∀'∀'(fn_domain ⟹ ∃'∀'(&0 ∈' &2 ⟹∀'(fn_app ↑' 1 # 2 ↑' 1 # 2 ⟹ (∀'(fn_app ↑' 1 # 1 ↑' 1 # 4 ↑' 1 # 4 ⊓ ∃'(&0 ∈' &2)) ⟹ &0 ∈' &1))))
+∃' ∀' ((is_emptyset.cast (lift_cast)  ⟹ (&0 ∈' &1) : bounded_formula L_ZFC 2) ⊓
+  (∀' (&0 ∈' &2 ⟹ (∃' ((&1 ∈' &0).cast (lift_cast) ⊓ (&0 ∈' &3) : bounded_formula L_ZFC 4)))))
 
 def axiom_of_emptyset : sentence L_ZFC := small ⊥
 -- todo: c can have free variables
 def axiom_of_separation (c : Class) : sentence L_ZFC := ∀' (small $ &0 ∈' &1 ⊓ c.cast1)
 -- the class consisting of the unordered pair {x, y}
 def axiom_of_pairing : sentence L_ZFC := ∀' ∀' small pair
+
+def ZF : Theory L_ZFC :=
+{axiom_of_extensionality, axiom_of_union, axiom_of_powerset, axiom_of_infinity} ∪
+(λ(c : bounded_formula L_ZFC 2), axiom_of_replacement c) '' set.univ
+
+local notation h :: t  := dvector.cons h t
+local notation `[` l:(foldr `, ` (h t, dvector.cons h t) dvector.nil `]`) := l
+
+def ordered_pair : bounded_formula L_ZFC 3 :=
+∀'(&0 ∈' &1 ⇔ (&0 ≃ &3 : bounded_formula L_ZFC 4) ⊔ ∀'(&0 ∈' &1 ⇔ pair ↑' 1 # 1 ↑' 1 # 1))
 --the class consisting of the ordered pair ⟨x, y⟩
 def axiom_of_ordered_pairing : sentence L_ZFC := ∀' ∀' small ordered_pair
 
-def ZF : Theory L_ZFC := {axiom_of_extensionality, axiom_of_union, axiom_of_powerset, axiom_of_infinity} ∪ (λ(c : bounded_formula L_ZFC 2), axiom_of_replacement c) '' set.univ
+-- &0 is an ordered pair of &2 and &1 (z = ⟨x, y⟩)
+
+def ordered_pair' : bounded_formula L_ZFC 3 :=
+∀'(&0 ∈' &3 ⇔ (&0 ≃ &2 : bounded_formula L_ZFC 4) ⊔ ∀'(&0 ∈' &1 ⇔ (pair ↑' 1 # 1).cast(lift_cast)))
+-- &2 is an ordered pair of &1 and &0 (x = ⟨y,z⟩)
+-- TODO: Make defns like this unnecessary (current effort is subst_var_* in fol.lean)
+
+def is_ordered_pair : bounded_formula L_ZFC 1 := ∃' ∃' ordered_pair
+--&0 is an ordered pair of some two elements--
+
+def relation : bounded_formula L_ZFC 1 := ∀' ((&0 ∈' &1) ⟹ is_ordered_pair ↑' 1 # 1)
+--&0 is a relation (is a set of ordered pairs)
+
+def relation' : bounded_formula L_ZFC 1 :=
+∀' (((&0 ∈' &1) : bounded_formula L_ZFC 2) ⟹ (is_ordered_pair ⊚ [0]))
+
+def function : bounded_formula L_ZFC 1 :=
+relation ⊓
+∀'∀'∀'∀'∀'(&1 ∈' &5 ⊓ ordered_pair ↑' 1 # 3 ↑' 1 # 1 ↑' 1 # 0 ⊓
+  ((&0 ∈' &5 : bounded_formula L_ZFC 6) ⊓ (ordered_pair ↑' 1 # 2 ↑' 1 # 1).cast(lift_cast)) ⟹
+    (&3 ≃ &2 : bounded_formula L_ZFC 6))
+-- X is a function iff X is a relation and the following holds:
+-- ∀x ∀y ∀z ∀w ∀t, ((w ∈ X) ∧ (w = ⟨x, y⟩) ∧ (z ∈ X) ∧ (z = ⟨x, z⟩ ))) → y = z
+
+def function' : bounded_formula L_ZFC 1 :=
+relation ⊓
+∀'∀'∀'∀'∀'(((&1 ∈' &5 : bounded_formula L_ZFC 6) ⊓ (ordered_pair ⊚ [1,3,4]) ⊓
+  ((&0 ∈' &5 : bounded_formula L_ZFC 6) ⊓ (ordered_pair ⊚ [0,2,4]))) ⟹
+    (&3 ≃ &2 : bounded_formula L_ZFC 6))
+
+def fn_app : bounded_formula L_ZFC 3 :=
+∃'(&0 ∈' &3 ⊓
+  ∀'(&0 ∈' &1 ⇔ ((&0 ≃ &3) : bounded_formula L_ZFC 5) ⊔ (pair ↑' 1 # 1).cast(lift_cast)))
+-- ⟨&1, &0⟩ ∈ &2
+-- &0 = &2(&1)
+
+def fn_domain : bounded_formula L_ZFC 2 :=
+∀'(&0 ∈' &2 ⇔ ∃'∃'(ordered_pair ↑' 1 # 1 ↑' 1 # 1 ⊓ &0 ∈' &3))
+-- &1 is the domain of &0
+
+def fn_range : bounded_formula L_ZFC 2 :=
+∀'(&0 ∈' &2 ⇔ ∃'∃'(∀'(&0 ∈' &1 ⇔ (&0 ≃ &2 : bounded_formula L_ZFC 6) ⊔
+  (pair ↑' 1 # 1).cast(lift_cast)) ⊓ &0 ∈' &3))
+--&1 is the range of &0
+
+def axiom_of_choice : sentence L_ZFC :=
+∀'∀'(fn_domain ⟹ ∃'∀'(&0 ∈' &2 ⟹∀'(fn_app ↑' 1 # 2 ↑' 1 # 2 ⟹
+  (∀'(fn_app ↑' 1 # 1 ↑' 1 # 4 ↑' 1 # 4 ⊓ ∃'(&0 ∈' &2)) ⟹ &0 ∈' &1))))
 
 def ZFC : Theory L_ZFC := ZF ∪ {axiom_of_choice}
 
+def inverse_relation : bounded_formula L_ZFC 2 :=
+∀'(&0 ∈' &1 ⇔ ∃'∃'(∃'(∀'(&0 ∈' &1 ⇔ (&0 ≃ &2 : bounded_formula L_ZFC 7) ⊔
+  (pair ↑' 1 # 1).cast(lift_cast)) ⊓ &0 ∈' &5 : bounded_formula L_ZFC 6)) ⊓
+  (ordered_pair'.cast(lift_cast)))
+-- &0 is the inverse relation of &1
+
+def function_one_one : bounded_formula L_ZFC 1 :=
+function ⊓ ∀' (inverse_relation ⟹ function.cast(lift_cast))
+
+def irreflexive_relation : bounded_formula L_ZFC 2 :=
+(∀'(&0 ∈' &2 ⟹ (∀'(∀'(&0 ∈' &1) ⇔ ((&0 ≃ &2 : bounded_formula L_ZFC 4) ⊔
+  ∀'(&0 ∈' &1 ⇔ (&0 ≃ &3 : bounded_formula L_ZFC 5))) ⟹ ∼(&0 ∈' &3))))) ⊓
+relation.cast(lift_cast)
+-- &0 is an irreflexive relation on &1
+
+def transitive_relation : bounded_formula L_ZFC 2 :=
+((∀'∀'∀'((((&2 ∈' &4 : bounded_formula L_ZFC 5) ⊓ (&1 ∈' &4)) ⊓ (&0 ∈' &4)) ⊓
+∃'((ordered_pair ↑' 1 # 1).cast(lift_cast) ⊓ (&0 ∈' &4 : bounded_formula L_ZFC 6)) ⊓
+∃'(ordered_pair.cast(lift_cast) ⊓ &0 ∈' &4 : bounded_formula L_ZFC 6) ⟹
+∃'((ordered_pair ↑' 1 # 2).cast(lift_cast) ⊓ &0 ∈' &4 : bounded_formula L_ZFC 6)))) ⊓
+relation.cast(lift_cast)
+--&0 is a transitive relation on &1
+-- X Tr Y iff X is a relation and the following holds:
+-- ∀u ∀v ∀w, (u ∈ Y ∧ v ∈ Y ∧ w ∈ Y ∧ ⟨u, v⟩ ∈ X ∧ ⟨v,w⟩ ∈ X) → ⟨u,w⟩ ∈ X
+
+def partial_order_zfc : bounded_formula L_ZFC 2 := irreflexive_relation ⊓ transitive_relation
+
+def connected_relation : bounded_formula L_ZFC 2 :=
+relation ↑' 1 # 1 ⊓ ∀'∀'((bd_and (bd_and (&0 ∈' &3) (&1 ∈' &3)) ∼(bd_equal &0 &1)) ⟹
+  ∃'((&0 ∈' &3 : bounded_formula L_ZFC 5) ⊓ ((ordered_pair ↑' 1 # 3 ↑' 1 # 3) ⊔
+  ∀'(&0 ∈' &1 ⇔ (&0 ≃ &2 : bounded_formula L_ZFC 6) ⊔ (pair ↑' 1 # 1).cast(lift_cast)))))
+--&0 is a connected relation on &1
+-- X Con Y iff Rel(X) and ∀u ∀v (u ∈ Y ∧ v ∈ Y ∧ u ≠ v) → ⟨u,v⟩ ∈ X ∨ ⟨v, u⟩ ∈ X
+
+def total_order : bounded_formula L_ZFC 2 :=
+irreflexive_relation ⊓ transitive_relation ⊓ connected_relation
+
+def well_order : bounded_formula L_ZFC 2 :=
+irreflexive_relation ⊓ ∀'(subset ↑' 1 # 1 ⊓ ∃'(&0 ∈' &1) ⟹ ∃'(&0 ∈' &1 ⊓
+∀'(((&0 ∈' &2) ⊓  ∼(&0 ≃ &1 : bounded_formula L_ZFC 5)) ⟹ ∃'(ordered_pair.cast(lift_cast) ⊓
+(&0 ∈' &4 : bounded_formula L_ZFC 6)) ⊓ ∼∃'(∀'(&0 ∈' &1 ⇔ (( &0 ≃ &2 : bounded_formula L_ZFC 7) ⊔
+(pair ↑' 1 # 1).cast(lift_cast) )) ⊓ &0 ∈' &4))))
+-- &0 well-orders &1
+
+def membership_relation : bounded_formula L_ZFC 1 :=
+relation ⊓
+  ∀'(&0 ∈' &1 ⇔ ∃'∃'∀'(&0 ∈' &3 ⇔ ((bd_equal &0  &2) ⊔ pair ↑' 1 # 3 ↑' 1 # 3) ⊓ &2 ∈' &1))
+-- &0 is E, the membership relation {⟨x,y⟩ | x ∈ y}
+
+def transitive_zfc : bounded_formula L_ZFC 1 := ∀' ((&0 ∈' &1) ⟹ subset)
+--&0 is transitive
+
+def fn_zfc_equiv : bounded_formula L_ZFC 3 :=
+((function_one_one.cast(lift_cast)) ⊓ (fn_domain ↑' 1 # 1)) ⊓ (fn_range ↑' 1 # 2)
+
+def zfc_equiv : bounded_formula L_ZFC 2 := ∃' fn_zfc_equiv
+--&0 ≃ &1, i.e. they are equinumerous
+
+def is_powerset : bounded_formula L_ZFC 2 := ∀' ((&0 ∈' &2) ⇔ subset ↑' 1 # 2)
+--&1 is P(&0)
+
+def is_suc_of : bounded_formula L_ZFC 2 :=
+∀' ((&0 ∈' &2) ⇔ ((&0 ∈' &1) ⊔ ( &0 ≃ &1 : bounded_formula L_ZFC 3)))
+-- &1 = succ(&0)
+
+def is_ordinal : bounded_formula L_ZFC 1 :=
+(∀' ((membership_relation.cast(lift_cast)) ⟹ well_order)) ⊓ transitive_zfc
+
+def is_suc_ordinal : bounded_formula L_ZFC 1 := is_ordinal ⊓ ∃' is_suc_of
+--&0 is a successor ordinal
+
+def ordinal_lt : bounded_formula L_ZFC 2 :=
+(is_ordinal.cast(lift_cast)) ⊓ (is_ordinal ↑' 1 # 0) ⊓ (&0 ∈' &1)
+-- &0 < &1
+
+def ordinal_le : bounded_formula L_ZFC 2 := ordinal_lt ⊔ (bd_equal &0 &1)
+-- &0 ≤ &1
+
+def is_first_infinite_ordinal : bounded_formula L_ZFC 1 :=
+∀' ((&0 ∈' &1) ⇔ (((is_emptyset ⊔ is_suc_ordinal)↑' 1 # 1) ⊓
+∀'((&0 ∈' &1) ⟹ ((is_emptyset ⊔ is_suc_ordinal).cast(lift_cast)))))
+--&0 = ω
+
+def is_uncountable_ordinal : bounded_formula L_ZFC 1 :=
+∀' ((is_first_infinite_ordinal.cast(lift_cast)) ⟹
+∀' (subset.cast(lift_cast) ⟹(∼(zfc_equiv ↑' 1 # 1))))
+--&0 ≥ ω₁
+
+def is_first_uncountable_ordinal : bounded_formula L_ZFC 1 :=
+is_uncountable_ordinal ⊓ (∀' ((is_uncountable_ordinal ↑' 1 # 1) ⟹ ordinal_le))
+--&0 = ω₁
+
+/- Statement of CH -/
+def continuum_hypothesis : sentence L_ZFC :=
+∀' ∀'  ((∃'((is_first_infinite_ordinal ↑' 1 # 1 ↑' 1 # 1) ⊓ (is_powerset ↑' 1 # 2)) ⊓
+  (is_first_uncountable_ordinal ↑' 1 #0)) ⟹ zfc_equiv)
 
 /- ZFC formulae in terms of Mario's Set type.
 Many of these are a lot shorter than the formulae above, largely because things like {x} and {{x},{x,y}} don't have to be existentially instantiated. It might be advantageous to refactor these to moatch the FOL formulae more precisely.
@@ -222,7 +273,8 @@ def Set_is_ordered_pair: Set → Prop := λ x, ∃ y z, Set_ordered_pair x y z
 
 def Set_relation : Set → Prop := λ x, ∀w, w ∈ x ↔ Set_is_ordered_pair w
 
-def Set_function : Set → Prop := λ x, Set_relation x ∧ ∀ a b c, ((({{a},{a,b}} ∈ x) ∧ ({{a},{a,c}} ∈ x)) → (b = c))
+def Set_function : Set → Prop :=
+λ x, Set_relation x ∧ ∀ a b c, ((({{a},{a,b}} ∈ x) ∧ ({{a},{a,c}} ∈ x)) → (b = c))
 
 def Set_fn_app : Set → Set → Set → Prop := λ x y z, {{x},{x,y}} ∈ z
 
@@ -232,31 +284,42 @@ def Set_fn_range: Set → Set → Prop := λ x y, ∀ w, w ∈ x ↔ ∃ a b, w 
 
 def Set_inverse_relation  : Set → Set → Prop := λ x y, ∀ a b, {{a},{a,b}} ∈ x ↔ {{b},{b,a}} ∈ y
 
-def Set_function_one_one : Set → Prop := λ x, Set_function x ∧ ∀ y, ((Set_inverse_relation x y) → Set_function y)
+def Set_function_one_one : Set → Prop :=
+λ x, Set_function x ∧ ∀ y, ((Set_inverse_relation x y) → Set_function y)
 
-def Set_irreflexive_relation : Set → Set → Prop := λ x y, Set_relation x ∧ ∀ z, z ∈ y → {{z},{z}} ∉ x
+def Set_irreflexive_relation : Set → Set → Prop :=
+λ x y, Set_relation x ∧ ∀ z, z ∈ y → {{z},{z}} ∉ x
 
-def Set_transitive_relation : Set → Set → Prop := λ x y, ∀ u v w, ((u ∈ y ∧ v ∈ y ∧ w ∈ w ∧ {{u},{u,v}} ∈ x ∧ {{v},{v,w}} ∈ x) → {{u},{u,w}} ∈ x)
+def Set_transitive_relation : Set → Set → Prop :=
+λ x y, ∀ u v w, ((u ∈ y ∧ v ∈ y ∧ w ∈ w ∧ {{u},{u,v}} ∈ x ∧ {{v},{v,w}} ∈ x) → {{u},{u,w}} ∈ x)
 
-def Set_partial_order : Set → Set → Prop := λ x y, Set_irreflexive_relation x y ⊓ Set_transitive_relation x y
+def Set_partial_order : Set → Set → Prop :=
+λ x y, Set_irreflexive_relation x y ⊓ Set_transitive_relation x y
 
-def Set_connected_relation: Set → Set → Prop := λ x y, Set_relation x ∧ ∀ u v, (u ∈ y ∧ v ∈ y ∧ u ≠ v) → ({{u},{u,v}} ∈ x ∨ {{v},{v,u}} ∈ x)
+def Set_connected_relation: Set → Set → Prop :=
+λ x y, Set_relation x ∧ ∀ u v, (u ∈ y ∧ v ∈ y ∧ u ≠ v) → ({{u},{u,v}} ∈ x ∨ {{v},{v,u}} ∈ x)
 
-def Set_total_order : Set → Set → Prop := λ X Y, (Set_irreflexive_relation X Y) ∧ (Set_transitive_relation X Y) ∧ (Set_connected_relation X Y)
+def Set_total_order : Set → Set → Prop :=
+λ X Y, (Set_irreflexive_relation X Y) ∧ (Set_transitive_relation X Y) ∧ (Set_connected_relation X Y)
 
-def Set_well_order : Set → Set → Prop := λ x y, Set_irreflexive_relation x y ∧ ∀ z, (z ⊆ y ∧ (z ≠ ∅) → ∃w, (w ∈ z ∧ ∀ v, ((v ∈ z ∧ v ≠ w) → {{w},{w,v}} ∈ x ∧ {{v},{v,w}} ∉ x)))
+def Set_well_order : Set → Set → Prop :=
+λ x y, Set_irreflexive_relation x y ∧
+∀ z, (z ⊆ y ∧ (z ≠ ∅) → ∃w, (w ∈ z ∧ ∀ v, ((v ∈ z ∧ v ≠ w) → {{w},{w,v}} ∈ x ∧ {{v},{v,w}} ∉ x)))
 
-def Set_membership_relation : Set → Prop := λ x, Set_relation x ∧ ∀ w ∈ x, ∃ u v, {{u},{u,v}} = w ∧ u ∈ v
+def Set_membership_relation : Set → Prop :=
+λ x, Set_relation x ∧ ∀ w ∈ x, ∃ u v, {{u},{u,v}} = w ∧ u ∈ v
 
 def Set_transitive : Set → Prop := λ x, ∀ w, w ∈ x → w ⊆ x
 
-def Set_fn_equiv : Set → Set → Set → Prop := λ x y z, Set_function_one_one x ∧ Set_fn_domain x y ∧ Set_fn_range x z
+def Set_fn_equiv : Set → Set → Set → Prop :=
+λ x y z, Set_function_one_one x ∧ Set_fn_domain x y ∧ Set_fn_range x z
 
 def Set_zfc_equiv : Set → Set → Prop := λ x y, ∃ f, Set_fn_equiv f x y
 
 def Set_is_suc_of : Set → Set → Prop := λ x y, ∀ w, (w ∈ x ↔ (w ∈ y ∨ w = y))
 
-def Set_is_ordinal : Set → Prop := λ x, (∀ w, (Set_membership_relation w → Set_well_order w x)) ∧ Set_transitive x
+def Set_is_ordinal : Set → Prop :=
+λ x, (∀ w, (Set_membership_relation w → Set_well_order w x)) ∧ Set_transitive x
 
 def Set_is_suc_ordinal : Set → Prop := λ x, Set_is_ordinal x ∧ ∃ w, Set_is_suc_of x w
 
@@ -264,19 +327,25 @@ def Set_ordinal_lt : Set → Set → Prop := λ x y, Set_is_ordinal x ∧ Set_is
 
 def Set_ordinal_le : Set → Set → Prop := λ x y, Set_ordinal_lt x y ∨ x = y
 
-def Set_is_first_infinite_ordinal : Set → Prop := λ x, ∀ w, (w ∈ x ↔ ((w = ∅ ∨ Set_is_suc_ordinal w) ∧ ∀ z, (z ∈ w → ((z = ∅ ∨ Set_is_suc_ordinal z)))))
+def Set_is_first_infinite_ordinal : Set → Prop :=
+λ x, ∀ w, w ∈ x ↔ ((w = ∅ ∨ Set_is_suc_ordinal w) ∧ ∀ z, (z ∈ w → (z = ∅ ∨ Set_is_suc_ordinal z)))
 
-def Set_is_uncountable_ordinal : Set → Prop := λ x, ∀ w, (Set_is_first_infinite_ordinal w → ∀ z, (Set.subset z w → ¬ Set_zfc_equiv z x))
+def Set_is_uncountable_ordinal : Set → Prop :=
+λ x, ∀ w, (Set_is_first_infinite_ordinal w → ∀ z, (Set.subset z w → ¬ Set_zfc_equiv z x))
 
-def Set_is_first_uncountable_ordinal : Set → Prop := λ x, Set_is_uncountable_ordinal x ∧ ∀ w, (Set_is_uncountable_ordinal w → Set_ordinal_le x w)
+def Set_is_first_uncountable_ordinal : Set → Prop :=
+λ x, Set_is_uncountable_ordinal x ∧ ∀ w, (Set_is_uncountable_ordinal w → Set_ordinal_le x w)
 
-def Set_continuum_hypothesis : Prop := ∀ x y, ((∃ w, (Set_is_first_infinite_ordinal w ∧ Set_is_powerset x w)) ∧ Set_is_first_uncountable_ordinal y) → Set_zfc_equiv x y
+def Set_continuum_hypothesis : Prop :=
+∀ x y, ((∃ w, (Set_is_first_infinite_ordinal w ∧ Set_is_powerset x w)) ∧
+  Set_is_first_uncountable_ordinal y) → Set_zfc_equiv x y
 
 --- shallow ZFC axioms
 
 def Set_axiom_of_infinity : Prop :=
 ∃ y : Set.{0}, ((∃ x : Set, (Set_is_emptyset x ∧ x ∈ y))∧ (∀ z, z ∈ y → (∃ w, z ∈ w ∧ w ∈ y) ))
 
-def Set_axiom_of_infinity' : Prop := ∃ y : Set.{0}, ∀ x : Set, ((Set_is_emptyset x → x ∈ y) ∧ ∀ z, z ∈ y → ∃ w, (z ∈ w) ∧ w ∈ y)
+def Set_axiom_of_infinity' : Prop :=
+∃ y : Set.{0}, ∀ x : Set, ((Set_is_emptyset x → x ∈ y) ∧ ∀ z, z ∈ y → ∃ w, (z ∈ w) ∧ w ∈ y)
 
 end zfc
